Cslib/Logics/NaturalDeduction/Realisability'.lean
@@ -1,0 +1,159 @@
+/-
+Copyright (c) 2025 Thomas Waring. All rights reserved.
+Released under Apache 2.0 license as described in the file LICENSE.
+Authors: Thomas Waring
+-/
+import Cslib.Logics.NaturalDeduction.NJ
+
+universe u v
+
+variable {Atom : Type u} [DecidableEq Atom]
+
+namespace IPL
+
+open Proposition
+
+namespace NJ
+
+open Derivation
+
+structure DerivationClosed (S : Set (Proposition Atom)) where
+  der {Γ : Ctx Atom} {B : Proposition Atom} (hΓ : ↑Γ ⊆ S) (hB : Derivable ⟨Γ, B⟩) : B ∈ S
+
+def Realiser : Proposition Atom → Type v
+  | atom _ => PUnit
+  | bot => PUnit
+  | conj A B => Realiser A × Realiser B
+  | disj A B => Realiser A ⊕ Realiser B
+  | impl A B => Realiser A → Realiser B
+
+def Realises (S : Set (Proposition Atom)) : (A : Proposition Atom) → Realiser A → Prop
+  | atom x, _ => atom x ∈ S
+  | bot, _ => False
+  | conj A B, t => Realises S A t.1 ∧ Realises S B t.2
+  | disj A _, Sum.inl x => Realises S A x
+  | disj _ B, Sum.inr y => Realises S B y
+  | impl A B, f => impl A B ∈ S ∧ ∀ x : Realiser A, Realises S A x → Realises S B (f x)
+
+theorem mem_gluing_of_realised (S : Set (Proposition Atom)) (hS : DerivationClosed S) :
+    (A : Proposition Atom) → (x : Realiser A) → Realises S A x → A ∈ S
+  | atom _, _, h => h
+  | bot, _, h => False.elim h
+  | conj A B, ⟨x, y⟩, ⟨hx, hy⟩ => by
+    refine hS.der (Γ := {A, B}) ?_ ?_
+    · have : A ∈ S := mem_gluing_of_realised S hS A x hx
+      have : B ∈ S := mem_gluing_of_realised S hS B y hy
+      grind
+    · exact ⟨conjI (A := A) (B := B) (ax' <| by grind) (ax' <| by grind)⟩
+  | disj A _, Sum.inl x, hx => by
+    refine hS.der (Γ := {A}) ?_ ?_
+    · have : A ∈ S := mem_gluing_of_realised S hS A x hx
+      grind
+    · exact ⟨disjI₁ (ax' <| by grind)⟩
+  | disj _ B, Sum.inr y, hy => by
+    refine hS.der (Γ := {B}) ?_ ?_
+    · have : B ∈ S := mem_gluing_of_realised S hS B y hy
+      grind
+    · exact ⟨disjI₂ (ax' <| by grind)⟩
+  | impl A B, _, ⟨h, _⟩ => h
+
+instance instInhabitedRealiser : (A : Proposition Atom) → Inhabited (Realiser A)
+  | atom _ => ⟨()⟩
+  | bot => ⟨()⟩
+  | conj A B =>
+    @instInhabitedProd _ _ (instInhabitedRealiser A) ((instInhabitedRealiser B))
+  | disj A _ => ⟨Sum.inl (instInhabitedRealiser A).default⟩
+  | impl _ B => @instInhabitedForall _ _ (instInhabitedRealiser B)
+
+def Derivation.Realiser {Γ : Ctx Atom} {B : Proposition Atom} (ts : ∀ A ∈ Γ, Realiser A) :
+    Derivation ⟨Γ, B⟩ → Realiser B
+  | ax Γ A => ts A (Finset.mem_insert_self A Γ)
+  | botE A _ => default
+  | conjI D E => ⟨D.Realiser ts, E.Realiser ts⟩
+  | conjE₁ D => (D.Realiser ts).1
+  | conjE₂ D => (D.Realiser ts).2
+  | disjI₁ D => Sum.inl <| D.Realiser ts
+  | disjI₂ D => Sum.inr <| D.Realiser ts
+  | @disjE _ _ Γ A B C D E₁ E₂ => by
+    cases D.Realiser ts
+    case inl t =>
+      refine E₁.Realiser ?_
+      intro A' hA'
+      by_cases A' ∈ Γ
+      case pos h => exact ts A' h
+      case neg h =>
+        have : A' = A := by grind
+        exact this ▸ t
+    case inr t =>
+      refine E₂.Realiser ?_
+      intro A' hA'
+      by_cases A' ∈ Γ
+      case pos h => exact ts A' h
+      case neg h =>
+        have : A' = B := by grind
+        exact this ▸ t
+  | @implI _ _ A B Γ D => by
+    intro tA
+    apply D.Realiser
+    intro A' hA'
+    by_cases A' ∈ Γ
+    case pos h => exact ts A' h
+    case neg h =>
+      have : A' = A := by grind
+      exact this ▸ tA
+  | implE D E => D.Realiser ts <| E.Realiser ts
+
+-- theorem adequacy (S : Set (Proposition Atom)) (Γ : Ctx Atom)
+--     (ts : ∀ A ∈ Γ, Realiser A) (hts : ∀ (A : Proposition Atom) (h : A ∈ Γ), Realises S A (ts A h))
+--     (B : Proposition Atom) (D : Derivation ⟨Γ, B⟩) : Realises S B <| D.Realiser ts := by
+--   cases D
+--   case ax Γ _ =>
+--     unfold Derivation.Realiser
+--     exact hts B (Finset.mem_insert_self B _)
+--   case botE D =>
+--     -- have : D.size < (botE B D).size := by grind [Derivation.size]
+--     exact False.elim <| adequacy S Γ ts hts bot D
+--   case conjI A B D E =>
+--     unfold Realises Derivation.Realiser
+--     reduce
+--     -- have : D.size < (conjI D E).size := by grind [Derivation.size]
+--     -- have : E.size < (conjI D E).size := by grind [Derivation.size]
+--     constructor <;> apply adequacy <;> exact hts
+--   case conjE₁ B' D =>
+--     -- have : D.size < (conjE₁ D).size := by grind [Derivation.size]
+--     have : _ := adequacy S Γ ts hts (B.conj B') D
+--     unfold Realises at this
+--     unfold Derivation.Realiser
+--     exact this.1
+--   case conjE₂ A D =>
+--     have : _ := adequacy S Γ ts hts (A.conj B) D
+--     unfold Realises at this
+--     unfold Derivation.Realiser
+--     exact this.2
+--   case disjI₁ A B D =>
+--     have :_ := adequacy S Γ ts hts A D
+--     unfold Realises Derivation.Realiser
+--     assumption
+--   case disjI₂ A B D =>
+--     have :_ := adequacy S Γ ts hts B D
+--     unfold Realises Derivation.Realiser
+--     assumption
+--   -- case disjE A A' D E E' =>
+--   --   unfold Derivation.Realiser
+--   --   cases D.Realiser ts
+
+--   termination_by D.size
+-- --   decreasing_by all_goals sorry
+-- --   -- · grind [Derivation.size]
+-- --   -- ·
+-- --   --   grind [Derivation.size]
+-- --   -- --   ·
+-- --     -- · expose_names
+-- --     --   -- rw [h_3]
+
+
+
+
+end NJ
+
+end IPL
