Cslib/Logics/NaturalDeduction/Realisability.lean
@@ -1,0 +1,139 @@
+/-
+Copyright (c) 2025 Thomas Waring. All rights reserved.
+Released under Apache 2.0 license as described in the file LICENSE.
+Authors: Thomas Waring
+-/
+import Cslib.Logics.NaturalDeduction.NJ
+import Mathlib.Computability.Primrec
+
+universe u v
+
+variable {Atom : Type u} [DecidableEq Atom]
+
+namespace IPL
+
+open Proposition
+
+namespace NJ
+
+open Derivation
+
+def Realiser (base : Atom → Type v) : Proposition Atom → Type v
+  | atom x => base x
+  | bot => PUnit
+  | conj A B => Realiser base A × Realiser base B
+  | disj A B => Realiser base A ⊕ Realiser base B
+  | impl A B => Realiser base A → Realiser base B
+
+structure IsGluingSet (base : Atom → Type v) (u : (x : Atom) → base x → Prop)
+    (S : Set (Proposition Atom)) where
+  atoms : ∀ (x : Atom), (∃ (t : base x), u x t) → atom x ∈ S
+  -- theorems : ∀ A : Proposition Atom, Proposition.PDerivable A → A ∈ S
+  der {Γ : Ctx Atom} {B : Proposition Atom} (hΓ : ↑Γ ⊆ S) (hB : Derivable ⟨Γ, B⟩) : B ∈ S
+  -- mp {A B : Proposition Atom} : (impl A B) ∈ S → A ∈ S → B ∈ S
+
+def Realises {base : Atom → Type v} (ρ : (x : Atom) → base x → Prop) (S : Set (Proposition Atom))
+    (hS : IsGluingSet base ρ S) : (A : Proposition Atom) → (Realiser base A) → Prop
+  | atom x, t => ρ x t
+  | bot, _ => False
+  | conj A B, ⟨s, t⟩ => Realises ρ S hS A s ∧ Realises ρ S hS B t
+  | disj A _, Sum.inl s => Realises ρ S hS A s
+  | disj _ B, Sum.inr t => Realises ρ S hS B t
+  | impl A B, f =>
+      impl A B ∈ S ∧ ∀ t : Realiser base A, Realises ρ S hS A t → Realises ρ S hS B (f t)
+
+theorem mem_gluing_of_realised {base : Atom → Type v} (ρ : (x : Atom) → base x → Prop)
+    (S : Set (Proposition Atom)) (hS : IsGluingSet base ρ S) (A : Proposition Atom)
+    (hA : ∃ t : Realiser base A, Realises ρ S hS A t) : A ∈ S := by
+  cases A <;> let ⟨t, ht⟩ := hA <;> unfold Realises at ht
+  case atom x =>
+    exact hS.atoms x ⟨t, ht⟩
+  case bot => contradiction
+  case conj A B =>
+    cases t
+    case mk s t =>
+      reduce at ht
+      have hA : A ∈ S := mem_gluing_of_realised ρ S hS A ⟨s, ht.1⟩
+      have hB : B ∈ S := mem_gluing_of_realised ρ S hS B ⟨t, ht.2⟩
+      apply hS.der (Γ := {A, B}) (B := A.conj B) (by grind)
+      constructor
+      apply conjI <;> exact ax' (by grind)
+  case disj A B =>
+    cases t
+    case inl s =>
+      reduce at ht
+      have hA : A ∈ S := mem_gluing_of_realised ρ S hS A ⟨s, ht⟩
+      apply hS.der (Γ := {A}) (B := A.disj B) (by grind)
+      constructor
+      apply disjI₁
+      exact ax' (by grind)
+    case inr t =>
+      reduce at ht
+      have hB : B ∈ S := mem_gluing_of_realised ρ S hS B ⟨t, ht⟩
+      apply hS.der (Γ := {B}) (B := A.disj B) (by grind)
+      constructor
+      apply disjI₂
+      exact ax' (by grind)
+  case impl A B => exact ht.1
+
+instance instInhabitedRealiser {base : Atom → Type v} (h_base : ∀ x : Atom, Inhabited (base x)) :
+    (A : Proposition Atom) → Inhabited (Realiser base A)
+  | atom x => h_base x
+  | bot => ⟨(default : PUnit)⟩
+  | conj A B =>
+      @instInhabitedProd _ _ (instInhabitedRealiser h_base A) ((instInhabitedRealiser h_base B))
+  | disj A _ => ⟨Sum.inl (instInhabitedRealiser h_base A).default⟩
+  | impl _ B => @instInhabitedForall _ _ (instInhabitedRealiser h_base B)
+
+def Derivation.Realiser {base : Atom → Type v} {Γ : Ctx Atom} {B : Proposition Atom}
+    (h_base : ∀ x : Atom, Inhabited (base x)) (ts : ∀ A ∈ Γ, Realiser base A) :
+    (D : Derivation ⟨Γ, B⟩) → Realiser base B
+  | ax Γ A => ts A (Finset.mem_insert_self A Γ)
+  | botE A _ => (instInhabitedRealiser h_base A).default
+  | conjI D E => ⟨D.Realiser h_base ts, E.Realiser h_base ts⟩
+  | conjE₁ D => (D.Realiser h_base ts).1
+  | conjE₂ D => (D.Realiser h_base ts).2
+  | disjI₁ D => Sum.inl <| D.Realiser h_base ts
+  | disjI₂ D => Sum.inr <| D.Realiser h_base ts
+  | @disjE _ _ Γ A B C D E₁ E₂ => by
+      cases D.Realiser h_base ts
+      case inl t =>
+        refine E₁.Realiser h_base ?_
+        intro A' hA'
+        by_cases A' ∈ Γ
+        case pos h => exact ts A' h
+        case neg h =>
+          have : A' = A := by grind
+          exact this ▸ t
+      case inr t =>
+        refine E₂.Realiser h_base ?_
+        intro A' hA'
+        by_cases A' ∈ Γ
+        case pos h => exact ts A' h
+        case neg h =>
+          have : A' = B := by grind
+          exact this ▸ t
+    | @implI _ _ A B Γ D => by
+        intro tA
+        apply D.Realiser h_base
+        intro A' hA'
+        by_cases A' ∈ Γ
+        case pos h => exact ts A' h
+        case neg h =>
+          have : A' = A := by grind
+          exact this ▸ tA
+    | implE D E => D.Realiser h_base ts <| E.Realiser h_base ts
+
+-- theorem adequacy {base : Atom → Type v} (ρ : (x : Atom) → base x → Prop)
+--     (S : Set (Proposition Atom)) (hS : IsGluingSet base ρ S)
+--     (h_base : ∀ x : Atom, Inhabited (base x)) (Γ : Ctx Atom) (ts : ∀ A ∈ Γ, Realiser base A)
+--     (hts : ∀ (A : Proposition Atom) (h : A ∈ Γ), Realises ρ S hS A (ts A h))
+--     (B : Proposition Atom) (D : Derivation ⟨Γ, B⟩) : Realises ρ S hS B <| D.Realiser h_base ts := by
+--   cases D
+--   case ax x =>
+--     unfold Derivation.Realiser
+--     sorry
+
+end NJ
+
+end IPL
